ex8wr.csh
@@ -1,0 +1,5 @@
+var ww: Ref[Num] = ref(0);
+fork {
+  *ww = 1;
+}
+var n: Num = *(ww);
