ex8ww.csh
@@ -1,0 +1,5 @@
+var ww: Ref[Num] = ref(0);
+fork {
+  *ww = 1;
+}
+*ww = 2;
